candle/standard/opentheory/readerProofScript.sml
@@ -1692,7 +1692,7 @@ val process_line_def = Define`
 
 val process_lines_def = Define`
   (process_lines fd st refs fs [] =
-    STDIO (add_stdout (fastForwardFD fs fd) (msg_success st)) *
+    STDIO (add_stdout (fastForwardFD fs fd) (msg_success st refs.the_context)) *
     HOL_STORE refs) ∧
   (process_lines fd st refs fs (ln::ls) =
    case process_line st refs ln of
@@ -1706,9 +1706,11 @@ val read_file_def = Define`
   read_file fs refs fnm =
     (if inFS_fname fs (File fnm) then
        (case readLines (all_lines fs (File fnm)) init_state refs of
-        | (Success (s,_), refs) => (T, add_stdout fs (msg_success s), refs)
+        | (Success (s,_), refs) =>
+            (T, add_stdout fs (msg_success s refs.the_context), refs)
         | (Failure (Fail e), refs) => (F, add_stderr fs e, refs))
-     else (F, add_stderr fs (msg_bad_name fnm), refs))`;
+     else
+       (F, add_stderr fs (msg_bad_name fnm), refs))`;
 
 val reader_main_def = Define `
    reader_main fs refs cl =
@@ -1742,25 +1744,13 @@ val process_line_inv = Q.store_thm("process_line_inv",
    \\ drule (GEN_ALL readLine_thm)
    \\ rpt (disch_then drule) \\ rw []);
 
-(* TODO
- * - print out the context in which the theorems were constructed.
- * - if we load holSoundnessTheory we can get semantic entailment also at
- *   the expense of a `is_set_theory mem' assumption.
- *)
-
 val reader_proves = Q.store_thm("reader_proves",
   `reader_main fs init_refs cl = (T,outp,refs)
    ==>
-   ?s defs.
-     (!asl c. MEM (Sequent asl c) s.thms ==>
-        (thyof defs, asl) |- c) /\
-     outp =
-       add_stdout fs
-         (concat
-           [strlit "OK! ";
-            concat [toString (LENGTH s.thms); strlit " theorems:\n"];
-            strlit "\n";
-            concat (MAP (λt. thm2str t ^ strlit "\n") s.thms)])`,
+   ?s ctxt.
+     (!asl c. MEM (Sequent asl c) s.thms ==> (thyof ctxt, asl) |- c) /\
+     outp = add_stdout fs (msg_success s ctxt) /\
+     ctxt extends init_ctxt`,
   rw [reader_main_def, case_eq_thms, read_file_def, bool_case_eq, PULL_EXISTS]
   \\ imp_res_tac init_reader_ok
   \\ `READER_STATE defs init_state` by fs [READER_STATE_init_state]
@@ -1769,7 +1759,9 @@ val reader_proves = Q.store_thm("reader_proves",
   \\ fs [READER_STATE_def, EVERY_MEM]
   \\ first_x_assum (assume_tac o REWRITE_RULE [THM_def] o
                     Q.GENL [`a`,`b`] o Q.SPEC `Sequent a b`)
-  \\ rw [msg_success_def]
+  \\ fs [STATE_def, CONTEXT_def] \\ rveq
+  \\ CONV_TAC SWAP_EXISTS_CONV
+  \\ qexists_tac `ds ++ refs'.the_context` \\ fs []
   \\ metis_tac []);
 
 val _ = export_theory();
